Refactoring

src/high/crash_weakestpre.v
@@ -14,14 +14,15 @@ Section wpc.
   Context `{nvmFixedG Σ, hGD : nvmDeltaG Σ}.
 
   (* NOTE: [R] is reflexive and hence we add the [s ≠ s'] in the conclusion. *)
-  Definition strictly_increasing_map (ss : gmap nat positive) (R : relation2 positive) :=
+  Definition strictly_increasing_map (R : relation2 positive) (ss : gmap nat positive) :=
     ∀ i j (s s' : positive),
       i < j → (ss !! i = Some s) → (ss !! j = Some s') → R s s' ∧ s ≠ s'.
 
-  Lemma strictly_increasing_map_singleton t s R : strictly_increasing_map {[ t := s ]} R.
+  Lemma strictly_increasing_map_singleton R t s :
+    strictly_increasing_map R {[ t := s ]}.
   Proof. intros ????? ?%lookup_singleton_Some ?%lookup_singleton_Some. lia. Qed.
 
-  Lemma strictly_increasing_map_empty  R : strictly_increasing_map ∅ R.
+  Lemma strictly_increasing_map_empty R : strictly_increasing_map R ∅.
   Proof. intros ????? [=]. Qed.
 
   (* Convert a message to a thread_view corresponding to what is stored in the
@@ -76,7 +77,7 @@ Section wpc.
       "exclusiveLocs" ∷ own exclusive_locs_name (● exclusive_locs) ∗
 
       "ordered" ∷ ([∗ map] ℓ ↦ hist; order ∈ abs_hists; orders,
-                    ⌜strictly_increasing_map hist order⌝) ∗
+                    ⌜strictly_increasing_map order hist⌝) ∗
 
       (* The predicates hold for all the exclusive locations. *)
       "map" ∷
